Proofs/Memory_Nodes.thy
@@ -16,20 +16,24 @@ abbreviation node_next
   where "node_next s n \<equiv> next_C (h_val (hrs_mem (t_hrs_' s)) n)" 
 abbreviation node_is_occupied
   where "node_is_occupied s n \<equiv> (mem_node_C.size_C (h_val (hrs_mem (t_hrs_' s)) n)) && scast  MEM_NODE_OCCUPIED_FLAG"
+
+abbreviation node_val
+  where "node_val s n \<equiv> (h_val (hrs_mem (t_hrs_' s)) n)"
     
 abbreviation update_node :: " globals \<Rightarrow> mem_node_C ptr \<Rightarrow> mem_node_C \<Rightarrow> globals"
-  where "update_node s n node_val \<equiv>
-  (t_hrs_'_update (hrs_mem_update (heap_update n node_val)) s)"
+  where "update_node s n new_val \<equiv>
+  (t_hrs_'_update (hrs_mem_update (heap_update n new_val)) s)"
 value t_hrs_'_update
   
 abbreviation hrs_the_same_at
   where "hrs_the_same_at s s' p \<equiv>
   fst (t_hrs_' s) p = fst (t_hrs_' s') p \<and> snd (t_hrs_' s) p = snd (t_hrs_' s') p"
+
 lemma t_hrs_'_t_hrs_'_update_simp:
   "t_hrs_' (t_hrs_'_update m (s::globals)) = m (t_hrs_' s)" by simp
     
 lemma updated_node_val: 
-  "h_val (hrs_mem (t_hrs_' (update_node s n node_val))) n = node_val"
+  "h_val (hrs_mem (t_hrs_' (update_node s n new_val))) n = new_val"
   by (simp add: h_val_heap_update hrs_mem_update)
     
 lemma updated_node_size:
@@ -41,15 +45,23 @@ lemma updated_node_next:
   using sable_isa.updated_node_val by auto
     
 lemma hrs_the_same_nodes_the_same:
-  "\<forall>p \<in> {ptr_val (node::mem_node_C ptr)..+size_of (TYPE(mem_node_C))}. hrs_the_same_at s s' p \<Longrightarrow>
-    (h_val (hrs_mem (t_hrs_' s)) node) = (h_val (hrs_mem (t_hrs_' s')) node)"
+  "\<forall>p \<in> ptr_span (node::mem_node_C ptr). hrs_the_same_at s s' p \<Longrightarrow>
+    node_val s node = node_val s' node"
   unfolding h_val_def hrs_mem_def
   apply (subgoal_tac " heap_list (fst (t_hrs_' s)) (size_of TYPE(mem_node_C)) (ptr_val node) =
      heap_list (fst (t_hrs_' s')) (size_of TYPE(mem_node_C)) (ptr_val node)")
    apply auto
   apply (rule heap_list_h_eq2)
   by simp
-    
+
+typ "heap_typ_desc" 
+typ "heap_mem"
+typ "heap_raw_state"
+
+value "t_hrs_'"
+value "hrs_mem"
+value "hrs_htd"
+  
 lemma MEM_NODE_OCCUPIED_FLAG_not_zero:
   "MEM_NODE_OCCUPIED_FLAG \<noteq> (0:: 32 signed word)" unfolding MEM_NODE_OCCUPIED_FLAG_def by auto
 
@@ -57,8 +69,11 @@ lemma one_mask_neg_MNOF_not_zero[simp]:
   "(1::32 signed word) && ~~ MEM_NODE_OCCUPIED_FLAG = (0::32 signed word) \<Longrightarrow> False"
      unfolding MEM_NODE_OCCUPIED_FLAG_def by unat_arith
 
-end
-  
+abbreviation
+  array_span :: "'a::mem_type ptr \<Rightarrow> nat \<Rightarrow> addr set" where
+  "array_span p arr_size \<equiv> {ptr_val p ..+ arr_size * size_of TYPE('a)}"
+
+end  
 end
   
   
